Cpc/Proofs/Rules/Str_in_re_sigma.lean
@@ -219,7 +219,7 @@ private theorem smtx_model_eval_str_in_re_sigma_rec
                     have hRv : rv = SmtRegLan.epsilon := by
                       change __smtx_model_eval M (SmtTerm.str_to_re (SmtTerm.String (native_string_lit ""))) =
                           SmtValue.RegLan rv at hREval
-                      rw [__smtx_model_eval.eq_104, __smtx_model_eval.eq_4] at hREval
+                      rw [__smtx_model_eval.eq_105, __smtx_model_eval.eq_4] at hREval
                       have hsimpa := hREval.symm
                       try simp [__smtx_model_eval_str_to_re, native_str_to_re, native_pack_string] at hsimpa ⊢
                       exact hsimpa
@@ -277,7 +277,7 @@ private theorem smtx_model_eval_str_in_re_sigma_rec
                           change __smtx_model_eval M
                               (SmtTerm.re_concat SmtTerm.re_allchar (__eo_to_smt x)) =
                             SmtValue.RegLan rv at hREval
-                          rw [__smtx_model_eval.eq_111, __smtx_model_eval.eq_101] at hREval
+                          rw [__smtx_model_eval.eq_112, __smtx_model_eval.eq_102] at hREval
                           cases hTailEval : __smtx_model_eval M (__eo_to_smt x) with
                           | RegLan rvTail =>
                               have hRv : rv = native_re_concat native_re_allchar rvTail := by
@@ -316,8 +316,8 @@ private theorem smtx_model_eval_str_in_re_sigma_rec
                                             (SmtTerm.re_mult SmtTerm.re_allchar)
                                             (__eo_to_smt x)) =
                                         SmtValue.RegLan rv at hREval
-                                      rw [__smtx_model_eval.eq_111, __smtx_model_eval.eq_105,
-                                        __smtx_model_eval.eq_101] at hREval
+                                      rw [__smtx_model_eval.eq_112, __smtx_model_eval.eq_106,
+                                        __smtx_model_eval.eq_102] at hREval
                                       cases hTailEval :
                                           __smtx_model_eval M (__eo_to_smt x) with
                                       | RegLan rvTail =>
@@ -502,7 +502,7 @@ private theorem smtx_model_eval_str_in_re_eq_sigma_side
       SmtValue.Boolean
         (nativeListInRe (native_unpack_string ss)
           (nativeSigmaState 0 true rv))
-  rw [__smtx_model_eval.eq_116]
+  rw [__smtx_model_eval.eq_117]
   have hState : nativeSigmaState 0 true rv = rv := by
     cases rv <;>
       simp [nativeSigmaState, nativeSigmaExact, native_re_mk_concat,
